\documentclass[12pt]{article}

\def\proof{{\it Proof.\ }}
\def\pf{{\hfill$\Box$}}

\newtheorem{thm}{Problem}

\usepackage{amssymb,graphicx}

\begin{document}

\noindent
{\bf\large Kim, Yie \& Yoo}

\noindent
{\bf MAT 512 Prof. Hurlbert}

\noindent
{\it Daily HW 8/29/09}
\vspace{0.5 in}

\begin{itemize}

\item[5]
\begin{thm}
Use three of the IMPORTANT IDENTITIES to prove that
$\displaystyle\sum\limits_{k=0}^{38204629939869} \frac {{{38204629939869}\choose{k}}}{{{76409259879737}\choose{k}}} = 2$

\end{thm}

\proof
Since numbers are too large, we try to generalize it. Both
two numbers are odd numbers with a relation 76409259879737 = 2 $\times$ 38204629939869 -1.
So the generalized version of this problem is to prove that $\displaystyle\sum\limits_{k=0}^{2m+1} \frac{{{2m+1} \choose {k}}}{{{4m+1 } \choose {k}}}= 2. $ \\	 
To prove generalied version of this problem, we use this identity\\

$\displaystyle\sum\limits_{i=0}^{k}{{n+i}\choose{i}} = {{n+k+i}\choose{k}} \cdot\cdot\cdot (*)$\\
              
Let's start\\\\
$\displaystyle\sum\limits_{k=0}^{2m+1} \frac{{{2m+1} \choose {k}}}{{{4m+1 } \choose {k}}}=  
1 + \sum\limits_{k=1}^{2m+1} \frac{{{2m+1} \choose {k}}}{{{4m+1 } \choose {k}}} \\
= 1 + \sum\limits_{k=1}^{2m+1} \frac{(4m+1-k)!(2m+1)!}{(2m+1-k)!(4m+1)!} \\
= 1 + \frac{(2m+1)!}{(4m+1)!}\sum\limits_{k=1}^{2m+1} \frac{(4m+1-k)!}{(2m+1-k)!} \\
= 1 + \frac{(2m+1)!}{(4m+1)!}\sum\limits_{k=1}^{2m+1} \frac{(4m+1-k)!(2m)!}{(2m+1-k)!(2m)!} \\
= 1 + \frac{(2m+1)!}{(4m+1)!}\sum\limits_{k=1}^{2m+1}{{4m+1-k}\choose{2m}} (2m)!\\
= 1 + \frac{(2m+1)!(2m)!}{(4m+1)!}\sum\limits_{k=1}^{2m+1}{{4m+1-k}\choose{2m}} \\
= 1 + \frac{1}{{{4m+1}\choose{2m}}}\sum\limits_{k=1}^{2m+1}{{4m+1-k}\choose{2m}} \\
= 1 + \frac{1}{{{4m+1}\choose{2m}}}\sum\limits_{i=0}^{2m}{{2m+i}\choose{i}} (by\ inverse\ order)\\
= 1 + \frac{1}{{{4m+1}\choose{2m}}}{{{4m+1}\choose{2m}}} (\because (*))\\
= 2
$	 

\pf

\end{itemize}

\end{document}
